Implement interpret_com and ni_com

fstar/Interpreter.fst
@@ -18,12 +18,57 @@ let rec interpret_exp env exp = match exp with
 	  | Times -> op_Multiply vleft vright
 
 
+type result =
+ | Finished : result
+ | OutOfFuel : result
+ | Error : result
+
+
+noeq type interpret_result =
+ | Result : result:result -> env:value_env -> fuel:nat -> interpret_result
+
+
+val interpret_com : value_env -> com -> nat -> interpret_result
+let rec interpret_com env com fuel = match com with
+ | Skip -> Result Finished env fuel
+ | Assign var exp -> Result Finished (update_env env var (interpret_exp env exp)) fuel
+ | Sequence c1 c2 -> let Result res env' fuel' = interpret_com env c1 fuel in
+                                              if res = OutOfFuel then
+											    Result res env' fuel'
+											  else
+												interpret_com env' c2 fuel'
+ | If cond thn els -> if (not (interpret_exp env cond = 0)) then
+                        interpret_com env thn fuel
+					  else
+                        interpret_com env els fuel
+ | While cond body -> if (not (interpret_exp env cond = 0)) then
+                        if fuel = 0 then
+						  Result OutOfFuel env fuel
+						else
+							let Result res env' fuel' = interpret_com env body fuel in
+												 if res = OutOfFuel then
+												   Result res env' fuel'
+												 else if fuel' = 0 then
+												   Result Error env' fuel'
+												 else if fuel' < fuel then
+												   interpret_com env' com (fuel' - 1)
+												 else
+												   Result Error env' fuel'
+                      else
+					    Result Finished env fuel
+
+
 type low_equiv (lenv:label_env) (e1:value_env) (e2:value_env) =
   forall (x:var). is_low lenv x ==> lookup_env e1 x == lookup_env e2 x
 
 type ni_exp (lenv:label_env) (exp:exp) =
   forall (e1:value_env) (e2:value_env). low_equiv lenv e1 e2 ==> interpret_exp e1 exp == interpret_exp e2 exp
 
+type res_equal (lenv:label_env) (r1:interpret_result) (r2:interpret_result) =
+  Result?.result r1 == Finished /\ Result?.result r2 == Finished ==> low_equiv lenv (Result?.env r1) (Result?.env r2)
+
+type ni_com (lenv:label_env) (com:com) =
+  forall (e1:value_env) (e2:value_env) (fuel1:nat) (fuel2:nat). low_equiv lenv e1 e2 ==> res_equal lenv (interpret_com e1 com fuel1) (interpret_com e2 com fuel2)
 
 val low_equiv_symmetric : lenv:label_env -> e1:value_env -> e2:value_env ->
   Lemma (requires (low_equiv lenv e1 e2))
@@ -71,6 +116,47 @@ val ni_binop : lenv:label_env -> op:binop -> exp1:exp -> exp2:exp ->
 let ni_binop _ _ _ _ = ()
 
 
+(*
+val ni_seq : lenv:label_env -> c1:com -> c2:com ->
+  lemma (requires (ni_com lenv c1 /\ ni_com lenv c2))
+        (ensures (ni_com lenv (sequence c1 c2)))
+let ni_seq lenv c1 c2 = ()
+*)
+
+val fuel_decr : env:value_env -> com:com -> fuel:nat ->
+  Lemma (requires (Result?.result (interpret_com env com fuel) = OutOfFuel))
+        (ensures (Result?.fuel (interpret_com env com fuel) = 0))
+let rec fuel_decr env com fuel = match com with
+ | Skip -> ()
+ | Assign _ _ -> ()
+ | If cond thn els ->
+					  if (not (interpret_exp env cond = 0)) then
+                        fuel_decr env thn fuel
+					  else
+                        fuel_decr env els fuel
+ | Sequence c1 c2 -> admit()
+ | _ -> admit()
+
+
+(*
+val ni_seq : lenv:label_env -> env:value_env -> fuel:nat -> c:com{Sequence? c} ->
+  Lemma (requires (ni_com lenv (Sequence?.s1 c) /\ ni_com lenv (Sequence?.s2 c)))
+        (ensures (ni_com lenv c))
+let ni_seq lenv env fuel c = match c with
+  | Sequence c1 c2 -> let r1 = interpret_com env fuel in
+                      let r2 = interpret_com env
+  assert (ni_com lenv c1);
+      assert (forall e1:value_env e2:value_env. interpret_exp lenv
+    assert (ni_com lenv c2);
+*)
+
+
+val typed_implies_ni : lenv:label_env -> com:com ->
+  Lemma (requires (typed_com lenv com Low))
+        (ensures (ni_com lenv com))
+let typed_implies_ni _ _ = admit()
+
+
 let _ =
 	let lenv = make_env Low [("lo", Low); ("lo2", Low); ("hi", High)] in
 
@@ -95,4 +181,33 @@ let _ =
 
 	assert (ni_exp lenv exp);
 	assert (ni_exp lenv exp');
-	assert (ni_exp lenv exp'')
+	assert (ni_exp lenv exp'');
+
+	assert (ni_com lenv Skip);
+	assert (ni_com lenv (Assign "lo" exp));
+
+	let not_ni_com = Assign "lo" (Var "hi") in
+	let env0 = make_env 0 [("lo", 0); ("hi", 0)] in
+	let env1 = make_env 0 [("lo", 0); ("hi", 1)] in
+
+	assert (low_equiv lenv env0 env1);
+
+	let r0 = interpret_com env0 not_ni_com 1 in
+	let r1 = interpret_com env1 not_ni_com 1 in
+
+	assert (Result?.result r0 = Finished);
+	assert (Result?.result r1 = Finished);
+
+	assert (lookup_env (Result?.env r0) "lo" = 0);
+	assert (lookup_env (Result?.env r1) "lo" = 1);
+
+	assert (~ (low_equiv lenv (Result?.env r0) (Result?.env r1)));
+	assert (~ (res_equal lenv r0 r1));
+
+	assert (~ (ni_com lenv not_ni_com));
+
+	let seq_com = (Sequence (Assign "hi" (Var "lo")) (Assign "lo" (Var "hi"))) in
+
+	assert (ni_com lenv seq_com);
+
+	()
