fstar/Label.fst
@@ -4,6 +4,7 @@ type label =
  | Low : label
  | High : label
 
+(*
 val op_Less : label -> label -> bool
 let op_Less l1 l2 = match l1, l2 with
  | Low, High -> true
@@ -11,6 +12,7 @@ let op_Less l1 l2 = match l1, l2 with
 
 val op_Less_Equals : label -> label -> bool
 let op_Less_Equals l1 l2 = l1 < l2 || l1 = l2
+*)
 
 val lub : label -> label -> label
 let lub l1 l2 = match l1, l2 with
